use ult instead sbb for Usubo for small cnf size

src/BBUsubo.v
@@ -1,6 +1,6 @@
-From Coq Require Import ZArith List.
+From Coq Require Import ZArith List Decidable.
 From mathcomp Require Import ssreflect ssrbool ssrnat eqtype seq tuple.
-From BitBlasting Require Import QFBVSimple CNF BBCommon BBNot BBAdd BBSub.
+From BitBlasting Require Import QFBVSimple CNF BBCommon BBUlt.
 From ssrlib Require Import Var ZAriths Tactics.
 From Bits Require Import bits.
 
@@ -11,13 +11,47 @@ Import Prenex Implicits.
 (* ===== bit_blast_usubo ===== *)
 
 Definition bit_blast_usubo w g (ls1 ls2: w.-tuple literal) : generator * cnf * literal :=
-  let '(g_sbb, cs_sbb, l_bout, lr_sbb) := bit_blast_sbb g lit_ff ls1 ls2 in
-  (g_sbb, cs_sbb, l_bout).
+  bit_blast_ult g ls1 ls2 .
 
 Definition mk_env_usubo w E g (ls1 ls2: w.-tuple literal) : env * generator * cnf * literal :=
-  let '(E_sbb, g_sbb, cs_sbb, l_bout, lr_sbb) := mk_env_sbb E g lit_ff ls1 ls2 in
-  (E_sbb, g_sbb, cs_sbb, l_bout).
+  mk_env_ult E g ls1 ls2.
 
+Lemma ltB_carry_subB:
+  forall w (bs1 bs2: BITS w),
+    ltB bs1 bs2 <->
+    carry_subB bs1 bs2.
+Proof.
+  move => w bs1 bs2.
+  split.
+  +
+    apply contrapositive.
+    - case: (carry_subB bs1 bs2);  rewrite /Decidable.decidable. by left. by right.
+    - move => Hinv_carry.
+      move /negP /eqP /eqP: Hinv_carry.
+      rewrite Bool.negb_true_iff => H.
+      move: (sbbB_ltB_leB bs1 bs2).
+      rewrite H /=.
+      move=> HleB HltB.
+      rewrite leBNlt in HleB.
+      move /negP : HleB => HleB.
+      rewrite HltB in HleB.
+      done.
+  +
+    move=> Hcarry.
+    move: (sbbB_ltB_leB bs1 bs2).
+    by rewrite Hcarry.
+Qed.
+
+Lemma ltB_carry_subB_rewrite:
+  forall w (bs1 bs2: BITS w),
+    ltB bs1 bs2 =
+    carry_subB bs1 bs2.
+Proof.
+  move=> w bs1 bs2.
+  case Hlt: (ltB bs1 bs2); case Hcarry: (carry_subB bs1 bs2); try done.
+  - apply ltB_carry_subB in Hlt. by rewrite Hlt in Hcarry.
+  - apply ltB_carry_subB in Hcarry. by rewrite Hcarry in Hlt.
+Qed.
 
 Lemma bit_blast_usubo_correct :
   forall w g (bs1 bs2 : BITS w) E ls1 ls2 br g' cs lr,
@@ -29,26 +63,21 @@ Lemma bit_blast_usubo_correct :
     enc_bit E lr br.
 Proof.
   move=> n g bs1 bs2 E ls1 ls2 br g' cs lrs.
-  rewrite /bit_blast_usubo. case HsbbB: (sbbB false bs1 bs2) => [obcout obrs].
-  case Hblast: (bit_blast_sbb g lit_ff ls1 ls2) => [[[og ocs] olcout] olrs].
+  rewrite /bit_blast_usubo.
+  case Hblast: (bit_blast_ult g ls1 ls2) => [[og ocs] olrs].
   case=> _ <- <- => Henc1 Henc2 <- Hcs.
-  move: (add_prelude_enc_bit_ff Hcs) => Hencff.
-  move: (bit_blast_sbb_correct Hblast Hencff Henc1 Henc2 Hcs HsbbB) => [H _].
-  done.
+  move: (bit_blast_ult_correct Hblast Henc1 Henc2 Hcs) => Henc.
+  by rewrite -(ltB_carry_subB_rewrite bs1 bs2).
 Qed.
+
+
 
 Lemma mk_env_usubo_is_bit_blast_usubo :
   forall w E g (ls1 ls2 : w.-tuple literal) E' g' cs lr,
     mk_env_usubo E g ls1 ls2 = (E', g', cs, lr) ->
     bit_blast_usubo g ls1 ls2 = (g', cs, lr).
 Proof.
-  move=> w E g ls1 ls2 E' g' cs lr.
-  rewrite /mk_env_usubo /bit_blast_usubo.
-  case Henv_sbb: (mk_env_sbb E g lit_ff ls1 ls2) => [[[[E_sbb g_sbb] cs_sbb] l_bout] lr_sbb].
-  case => _ <- <- <-.
-  dcase_goal.
-  move: (mk_env_sbb_is_bit_blast_sbb Henv_sbb).
-  by rewrite H; case => <- <- <- _.
+  exact: (mk_env_ult_is_bit_blast_ult).
 Qed.
 
 Lemma mk_env_usubo_newer_gen :
@@ -56,10 +85,7 @@ Lemma mk_env_usubo_newer_gen :
     mk_env_usubo E g ls1 ls2 = (E', g', cs, lr) ->
     (g <=? g')%positive.
 Proof.
-  move=> w E g ls1 ls2 E' g' cs lr. rewrite /mk_env_usubo.
-  dcase (mk_env_sbb E g lit_ff ls1 ls2) => [[[[[E_sbb g_sbb] cs_sbb] l_bout] lrs_sbb] Henv_sbb].
-  case=> _ <- _ _.
-  exact: (mk_env_sbb_newer_gen Henv_sbb).
+  exact: (mk_env_ult_newer_gen).
 Qed.
 
 Lemma mk_env_usubo_newer_res :
@@ -68,10 +94,7 @@ Lemma mk_env_usubo_newer_res :
     newer_than_lit g lit_tt ->
     newer_than_lit g' lr.
 Proof.
-  move=> w E g ls1 ls2 E' g' cs lr. rewrite /mk_env_usubo.
-  dcase (mk_env_sbb E g lit_ff ls1 ls2) => [[[[[E_sbb g_sbb] cs_sbb] l_bout] lrs_sbb] Henv_sbb].
-  case=> _ <- _ <- Hgtt.
-  exact: (mk_env_sbb_newer_bout Henv_sbb Hgtt).
+  exact: (mk_env_ult_newer_res).
 Qed.
 
 
@@ -83,10 +106,7 @@ Lemma mk_env_usubo_newer_cnf :
     newer_than_lits g ls2 ->
     newer_than_cnf g' cs.
 Proof.
-  move=> w E g ls1 ls2 E' g' cs lr. rewrite /mk_env_usubo.
-  dcase (mk_env_sbb E g lit_ff ls1 ls2) => [[[[[E_sbb g_sbb] cs_sbb] l_bout] lrs_sbb] Henv_sbb].
-  case=> _ <- <- _. move=> Hnew_gtt Hnew_gls1 Hnew_gls2.
-  exact: (mk_env_sbb_newer_cnf Henv_sbb Hnew_gtt Hnew_gls1 Hnew_gls2).
+  exact: (mk_env_ult_newer_cnf).
 Qed.
 
 Lemma mk_env_usubo_preserve :
@@ -94,10 +114,7 @@ Lemma mk_env_usubo_preserve :
     mk_env_usubo E g ls1 ls2 = (E', g', cs, lr) ->
     env_preserve E E' g.
 Proof.
-  move=> w E g ls1 ls2 E' g' cs lr. rewrite /mk_env_usubo.
-  dcase (mk_env_sbb E g lit_ff ls1 ls2) => [[[[[E_sbb g_sbb] cs_sbb] l_bout] lrs_sbb] Henv_sbb].
-  case=> <- _ _ _.
-  exact: (mk_env_sbb_preserve Henv_sbb).
+  exact: (mk_env_ult_preserve).
 Qed.
 
 Lemma mk_env_usubo_sat :
@@ -108,8 +125,5 @@ Lemma mk_env_usubo_sat :
     newer_than_lits g ls2 ->
     interp_cnf E' cs.
 Proof.
-  move=> w E g ls1 ls2 E' g' cs lr. rewrite /mk_env_usubo.
-  dcase (mk_env_sbb E g lit_ff ls1 ls2) => [[[[[E_sbb g_sbb] cs_sbb] l_bout] lrs_sbb] Henv_sbb].
-  case=> <- _ <- _. move=> Hnew_gtt Hnew_gls1 Hnew_gls2.
-  exact: (mk_env_sbb_sat Henv_sbb Hnew_gtt Hnew_gls1 Hnew_gls2).
+  exact: (mk_env_ult_sat).
 Qed.
